hol/p4_exec_sem_stmt_soundnessScript.sml
@@ -26,18 +26,6 @@ Definition frame_list_exec_sound:
   frames_red ctx (g_scope_list, frame_list, ctrl, status) state')
 End
 
-(* TODO: This could be used to remove if-statements in the executable semantics
-Theorem stmt_exec_funn_inv:
-!ctx g_scope_list funn stmt_stack scopes_stack ctrl status g_scope_list' funn' stmt_stack' scopes_stack' ctrl' status' frame'. 
-(stmt_exec ctx (g_scope_list, [(funn, stmt_stack, scopes_stack)], ctrl, status) =
- SOME (g_scope_list', [(funn', stmt_stack', scopes_stack')], ctrl', status') ==> funn = funn') /\
-(stmt_exec ctx (g_scope_list, [(funn, stmt_stack, scopes_stack)], ctrl, status) =
- SOME (g_scope_list', [frame'; (funn', stmt_stack', scopes_stack')], ctrl', status') ==> funn = funn')
-Proof
-cheat
-QED
-*)
-
 (*
 val specl_stmt_block_exec_empty =
  SIMP_RULE list_ss [] (ISPECL [``ctx:ctx``, ``g_scope_list:g_scope_list``, ``funn:funn``, ``s:stmt``, ``scopes_stack:scopes_stack``, ``ctrl:ctrl``, ``status_running``, ``g_scope_list':g_scope_list``, ``[]:frame_list``] ((valOf o find_clause_stmt_red) "stmt_block_exec"))
@@ -58,16 +46,18 @@ Cases_on `status` >> (
 ) >>
 pairLib.PairCases_on `ctx` >>
 rename1 `(ext_map, func_map, b_func_map, pars_map, tbl_map)` >>
-fs [stmt_exec] >>
+Cases_on `scopes_stack` >> (
+ fs [stmt_exec]
+) >>
 Cases_on `lookup_ext_fun funn ext_map` >> (
  fs []
 ) >>
-Cases_on `x (g_scope_list,scopes_stack,ctrl)` >> (
+Cases_on `x (g_scope_list,h::t,ctrl)` >> (
  fs []
 ) >>
 pairLib.PairCases_on `x'` >>
 fs [] >>
-METIS_TAC [(valOf o find_clause_stmt_red) "stmt_ext", clause_name_def]
+metis_tac [(valOf o find_clause_stmt_red) "stmt_ext", clause_name_def]
 QED
 
 Theorem stmt_ret_exec_sound_red:
@@ -80,21 +70,24 @@ rpt strip_tac >>
 Cases_on `status` >> (
  fs [stmt_exec]
 ) >>
+Cases_on `scopes_stack` >> (
+ fs [stmt_exec]
+) >>
 Cases_on `get_v e` >> (
  fs []
 ) >| [
- Cases_on `e_exec ctx g_scope_list scopes_stack e` >> (
+ Cases_on `e_exec ctx g_scope_list (h::t) e` >> (
   fs []
  ) >>
  Cases_on `x` >> (
   fs []
  ) >>
- METIS_TAC [(valOf o find_clause_stmt_red) "stmt_ret_e", clause_name_def],
+ metis_tac [(valOf o find_clause_stmt_red) "stmt_ret_e", clause_name_def],
 
  Cases_on `e` >> (
   fs [get_v]
  ) >>
- METIS_TAC [(valOf o find_clause_stmt_red) "stmt_ret_v", clause_name_def]
+ metis_tac [(valOf o find_clause_stmt_red) "stmt_ret_v", clause_name_def]
 ]
 QED
 
@@ -108,6 +101,9 @@ rpt strip_tac >>
 Cases_on `status` >> (
  fs [stmt_exec]
 ) >>
+Cases_on `scopes_stack` >> (
+ fs [stmt_exec]
+) >>
 Cases_on `is_v e` >> (
  fs []
 ) >| [
@@ -119,14 +115,14 @@ Cases_on `is_v e` >> (
  ) >>
  rw [] >>
  fs [stmt_exec_trans] >>
- METIS_TAC [(valOf o find_clause_stmt_red) "stmt_trans", clause_name_def],
+ metis_tac [(valOf o find_clause_stmt_red) "stmt_trans", clause_name_def],
 
- Cases_on `e_exec ctx g_scope_list scopes_stack e` >> (
+ Cases_on `e_exec ctx g_scope_list (h::t) e` >> (
   fs []
  ) >>
  pairLib.PairCases_on `x` >>
  fs [] >>
- METIS_TAC [(valOf o find_clause_stmt_red) "stmt_trans_e", clause_name_def]
+ metis_tac [(valOf o find_clause_stmt_red) "stmt_trans_e", clause_name_def]
 ]
 QED
 
@@ -144,10 +140,12 @@ rename1 `(ext_map, func_map, b_func_map, pars_map, tbl_map)` >>
 Cases_on `status` >> (
  fs [stmt_exec]
 ) >>
+Cases_on `scopes_stack` >> (
+ fs [stmt_exec]
+) >>
 Cases_on `index_not_const e_l` >> (
  fs []
 ) >| [
- (* TODO: stmt_apply_table_v *)
  Cases_on `FLOOKUP tbl_map tbl` >> (
   fs []
  ) >>
@@ -157,38 +155,35 @@ Cases_on `index_not_const e_l` >> (
  pairLib.PairCases_on `x'` >>
  fs [] >>
  rw [] >>
- cheat,
-
- (* TODO: stmt_apply_table_e *)
- cheat
-]
-(* OLD:
-Cases_on `get_v e` >> (
- fs []
-) >| [
- Cases_on `e_exec (ext_map, func_map, tbl_map) g_scope_list scopes_stack e` >> (
-  fs []
+ IMP_RES_TAC index_not_const_NONE >>
+ subgoal `?v_l. x'1 = MAP e_v v_l` >- (
+  qexists_tac `vl_of_el x'1` >>
+  IMP_RES_TAC vl_of_el_MAP_e_v
  ) >>
- pairLib.PairCases_on `x` >>
- fs [] >>
- METIS_TAC [(valOf o find_clause_stmt_red) "stmt_apply_table_e", clause_name_def],
+ Q.SUBGOAL_THEN `(MAP ( \ (e_,mk_). e_) (ZIP (e_l,x)) = e_l) /\
+                 (MAP ( \ v_. e_v v_) v_l = x'1)`
+  (fn thm => (irule (SIMP_RULE std_ss [thm] (ISPECL [``ZIP ((e_l:e list), x: mk list)``, ``v_l:v list``]
+                                                  ((valOf o find_clause_stmt_red) "stmt_apply_table_v"))))) >- (
+  fs [lambda_FST, MAP_ZIP] >>
+  metis_tac []
+ ) >>
+ fs [clause_name_def, lambda_SND, MAP_ZIP],
 
- Cases_on `FLOOKUP tbl_map s` >> (
+ Cases_on `e_exec (ext_map,func_map,b_func_map,pars_map,tbl_map) g_scope_list (h::t) (EL x e_l)` >> (
   fs []
  ) >>
  pairLib.PairCases_on `x'` >>
  fs [] >>
- Cases_on `ctrl (s,x,x'1)` >> (
-  fs []
+ rw [] >>
+ Q.SUBGOAL_THEN `(MAP ( \ (e_,e'_). e_) (ZIP ((e_l:e list), (LUPDATE x'0 x e_l):e list)) = e_l) /\
+                 (MAP ( \ (e_,e'_). e'_) (ZIP ((e_l:e list), (LUPDATE x'0 x e_l):e list)) = (LUPDATE x'0 x e_l))`
+  (fn thm => (irule (SIMP_RULE std_ss [thm] (ISPEC ``ZIP ((e_l:e list), (LUPDATE x'0 x e_l):e list)``
+                                                  ((valOf o find_clause_stmt_red) "stmt_apply_table_e"))))) >- (
+  fs [lambda_FST, lambda_SND, MAP_ZIP]
  ) >>
- pairLib.PairCases_on `x'` >>
- fs [] >>
- Cases_on `e` >> (
-  fs [get_v]
- ) >>
- METIS_TAC [(valOf o find_clause_stmt_red) "stmt_apply_table_v", clause_name_def]
+ fs [clause_name_def] >>
+ metis_tac [e_exec_sound]
 ]
-*)
 QED
 
 Theorem stmt_verify_exec_sound_red:
@@ -198,77 +193,44 @@ e_exec_sound e2 ==>
 stmt_exec_sound (stmt_verify e1 e2)
 Proof
 fs [stmt_exec_sound, e_exec_sound] >>
-REPEAT STRIP_TAC >>
+rpt strip_tac >>
 pairLib.PairCases_on `state'` >>
 rename1 `(g_scope_list',state'1,state'2,state'3)` >>
 rename1 `(g_scope_list',frame_list',ctrl',status')` >>
 Cases_on `status` >> (
  fs [stmt_exec]
 ) >>
+fs [exec_stmt_verify_SOME_REWRS] >>
 Cases_on `is_v e1` >> Cases_on `is_v e2` >| [
  (* First case *)
- fs [] >>
- Cases_on `stmt_exec_verify e1 e2` >> (
-  fs [] >>
-  rw []
- ) >>
  Cases_on `e1` >> Cases_on `e2` >> (
-  fs [stmt_exec_verify] >>
-  rw []
+  fs [stmt_exec_verify]
  ) >>
- rename1 `is_v_bool (e_v v1)` >>
- rename1 `is_v_err (e_v v2)` >>
- Cases_on `v1` >> Cases_on `v2` >> (
-  fs [stmt_exec_verify] >>
-  rw []
+ Cases_on `v` >> Cases_on `v'` >> (
+  fs [stmt_exec_verify]
  ) >>
- Cases_on `x` >> (
-  Cases_on `b` >> (
-   fs [stmt_exec_verify]
-  )
+ Cases_on `b` >> (
+  fs [stmt_exec_verify]
  ) >| [
-  METIS_TAC [(valOf o find_clause_stmt_red) "stmt_verify_3", clause_name_def],
+  metis_tac [(valOf o find_clause_stmt_red) "stmt_verify_3", clause_name_def],
 
-  METIS_TAC [(valOf o find_clause_stmt_red) "stmt_verify_4", clause_name_def]
+  metis_tac [(valOf o find_clause_stmt_red) "stmt_verify_4", clause_name_def]
  ],
 
  (* Second case - second operand unreduced *)
- fs [] >>
- Cases_on `e_exec ctx g_scope_list scopes_stack e2` >> (
-  fs []
- ) >>
- Cases_on `x` >>
- fs [] >>
- rw [] >>
  Cases_on `e1` >> (
-  fs [is_v] >>
-  rw []
+  fs [is_v]
  ) >>
  Cases_on `v` >> (
-  fs [is_v_bool] >>
-  rw []
+  fs [is_v_bool]
  ) >>
- METIS_TAC [((valOf o find_clause_stmt_red) "stmt_verify_e2"), clause_name_def],
+ metis_tac [((valOf o find_clause_stmt_red) "stmt_verify_e2"), clause_name_def],
 
  (* Third case - first operand unreduced *)
- fs [] >>
- Cases_on `e_exec ctx g_scope_list scopes_stack e1` >> (
-  fs []
- ) >>
- Cases_on `x` >>
- fs [] >>
- rw [] >>
- METIS_TAC [((valOf o find_clause_stmt_red) "stmt_verify_e1"), clause_name_def],
+ metis_tac [((valOf o find_clause_stmt_red) "stmt_verify_e1"), clause_name_def],
 
  (* Fourth case - both operands unreduced *)
- fs [] >>
- Cases_on `e_exec ctx g_scope_list scopes_stack e1` >> (
-  fs []
- ) >>
- Cases_on `x` >>
- fs [] >>
- rw [] >>
- METIS_TAC [((valOf o find_clause_stmt_red) "stmt_verify_e1"), clause_name_def]
+ metis_tac [((valOf o find_clause_stmt_red) "stmt_verify_e1"), clause_name_def]
 ]
 QED
 
@@ -282,10 +244,13 @@ rpt strip_tac >>
 Cases_on `status` >> (
  fs [stmt_exec]
 ) >>
+Cases_on `scopes_stack` >> (
+ fs [stmt_exec]
+) >>
 Cases_on `is_v e` >> (
  fs []
 ) >| [
- Cases_on `stmt_exec_ass lval e (g_scope_list ++ scopes_stack)` >> (
+ Cases_on `stmt_exec_ass lval e (g_scope_list ++ (h::t))` >> (
   fs []
  ) >>
  Cases_on `e` >> (
@@ -311,24 +276,24 @@ Cases_on `is_v e` >> (
   Cases_on `g_scope_list'` >> (
    fs []
   ) >>
-  Cases_on `t` >> (
+  Cases_on `t'` >> (
    fs []
   ),
 
   Cases_on `g_scope_list'` >> (
    fs []
   ) >>
-  Cases_on `t` >> (
+  Cases_on `t'` >> (
    fs []
   )
  ],
 
- Cases_on `e_exec ctx g_scope_list scopes_stack e` >> (
+ Cases_on `e_exec ctx g_scope_list (h::t) e` >> (
   fs []
  ) >>
  pairLib.PairCases_on `x` >>
  fs [] >>
- METIS_TAC [((valOf o find_clause_stmt_red) "stmt_ass_e"), clause_name_def]
+ metis_tac [((valOf o find_clause_stmt_red) "stmt_ass_e"), clause_name_def]
 ]
 QED
 
@@ -343,15 +308,18 @@ rpt strip_tac >>
 Cases_on `status` >> (
  fs [stmt_exec]
 ) >>
+Cases_on `scopes_stack` >> (
+ fs [stmt_exec]
+) >>
 Cases_on `is_empty s1` >> (
  fs []
 ) >| [
  Cases_on `s1` >> (
   fs [is_empty]
  ) >>
- METIS_TAC [((valOf o find_clause_stmt_red) "stmt_seq2"), clause_name_def],
+ metis_tac [((valOf o find_clause_stmt_red) "stmt_seq2"), clause_name_def],
 
- Cases_on `stmt_exec ctx (g_scope_list,[(funn,[s1],scopes_stack)],ctrl,status_running)` >> (
+ Cases_on `stmt_exec ctx (g_scope_list,[(funn,[s1],(h::t))],ctrl,status_running)` >> (
   fs []
  ) >>
  pairLib.PairCases_on `x` >> (
@@ -360,16 +328,16 @@ Cases_on `is_empty s1` >> (
  Cases_on `x1` >> (
   fs []
  ) >>
- Cases_on `t` >> (
+ Cases_on `t'` >> (
   fs []
  ) >| [
-  pairLib.PairCases_on `h` >> (
+  pairLib.PairCases_on `h'` >> (
    fs []
   ) >>
-  Cases_on `h1` >> (
+  Cases_on `h'1` >> (
    fs []
   ) >>
-  Cases_on `t` >> (
+  Cases_on `t'` >> (
    fs []
   ) >| [
    Cases_on `x3` >> (
@@ -378,10 +346,9 @@ Cases_on `is_empty s1` >> (
     rw [] >>
     rename1 `(x0, [(funn', [stmt_seq s1' s2], scopes_stack')], ctrl', status_running)` >>
     rename1 `(g_scope_list', [(funn', [stmt_seq s1' s2], scopes_stack')], ctrl', status_running)` >>
-    (* TODO *)
     Q.SUBGOAL_THEN `funn' = funn`
      (fn thm => fs [thm]) >- (
-     cheat
+     metis_tac [stmt_exec_inv]
     ) >>
     Q.SUBGOAL_THEN `[(funn, [stmt_seq s1' s2], scopes_stack')] = [] ++ [(funn, [stmt_seq s1' s2], scopes_stack')]`
      (fn thm => ONCE_REWRITE_TAC [thm]) >- (
@@ -397,64 +364,60 @@ Cases_on `is_empty s1` >> (
     rw [] >>
     rename1 `(x0, [(funn', [s], scopes_stack')], ctrl', status_returnv v)` >>
     rename1 `(g_scope_list', [(funn', [s], scopes_stack')], ctrl', status_returnv v)` >>
-    (* TODO *)
     Q.SUBGOAL_THEN `funn' = funn`
      (fn thm => fs [thm]) >- (
-     cheat
+     metis_tac [stmt_exec_inv]
     ) >>
-    METIS_TAC [((valOf o find_clause_stmt_red) "stmt_seq3"), clause_name_def, status_distinct],
+    metis_tac [((valOf o find_clause_stmt_red) "stmt_seq3"), clause_name_def, status_distinct],
 
     rw [] >>
     rename1 `(x0, [(funn', [s1'], scopes_stack')], ctrl', status_trans s)` >>
     rename1 `(g_scope_list', [(funn', [s1'], scopes_stack')], ctrl', status_trans s)` >>
-    (* TODO *)
     Q.SUBGOAL_THEN `funn' = funn`
      (fn thm => fs [thm]) >- (
-     cheat
+     metis_tac [stmt_exec_inv]
     ) >>
-    METIS_TAC [((valOf o find_clause_stmt_red) "stmt_seq3"), clause_name_def, status_distinct],
+    metis_tac [((valOf o find_clause_stmt_red) "stmt_seq3"), clause_name_def, status_distinct],
 
     rw [] >>
     rename1 `(x0, [(funn', [s1'], scopes_stack')], ctrl', status_type_error)` >>
     rename1 `(g_scope_list', [(funn', [s1'], scopes_stack')], ctrl', status_type_error)` >>
-    (* TODO *)
     Q.SUBGOAL_THEN `funn' = funn`
      (fn thm => fs [thm]) >- (
-     cheat
+     metis_tac [stmt_exec_inv]
     ) >>
-    METIS_TAC [((valOf o find_clause_stmt_red) "stmt_seq3"), clause_name_def, status_distinct]
+    metis_tac [((valOf o find_clause_stmt_red) "stmt_seq3"), clause_name_def, status_distinct]
    ],
 
-   Cases_on `h'` >> (
-    fs []
-   ) >>
-   Cases_on `t'` >> (
+   Cases_on `t''` >> (
     fs []
    ) >>
    Cases_on `x3` >> (
     fs []
    ) >>
    rw [] >>
-   (* TODO: seq1? *)
+   (* TODO: stmt_seq1 *)
+   (* ((valOf o find_clause_stmt_red) "stmt_seq1") *)
    cheat
   ],
 
-  pairLib.PairCases_on `h'` >> (
+  pairLib.PairCases_on `h''` >> (
    fs []
   ) >>
-  Cases_on `h'1` >> (
-   fs []
-  ) >>
-  Cases_on `t` >> (
+  Cases_on `h''1` >> (
    fs []
   ) >>
   Cases_on `t'` >> (
    fs []
   ) >>
+  Cases_on `t''` >> (
+   fs []
+  ) >>
   Cases_on `x3` >> (
    fs []
   ) >>
-  (* TODO: seq1? *)
+  (* TODO: seq1: new frame is created *)
+  rw [] >>
   cheat
  ]
 ]
@@ -480,11 +443,11 @@ Cases_on `is_empty s1` >> (
    irule ((valOf o find_clause_stmt_red) "stmt_seq1") >>
    fs [clause_name_def],
 
-   METIS_TAC [((valOf o find_clause_stmt_red) "stmt_seq3"), clause_name_def, status_distinct],
+   metis_tac [((valOf o find_clause_stmt_red) "stmt_seq3"), clause_name_def, status_distinct],
 
-   METIS_TAC [((valOf o find_clause_stmt_red) "stmt_seq3"), clause_name_def, status_distinct],
+   metis_tac [((valOf o find_clause_stmt_red) "stmt_seq3"), clause_name_def, status_distinct],
 
-   METIS_TAC [((valOf o find_clause_stmt_red) "stmt_seq3"), clause_name_def, status_distinct]
+   metis_tac [((valOf o find_clause_stmt_red) "stmt_seq3"), clause_name_def, status_distinct]
   ],
 
   pairLib.PairCases_on `h'` >>
@@ -516,7 +479,7 @@ stmt_exec_sound (stmt_cond e s1 s2)
 Proof
 fs [stmt_exec_sound, e_exec_sound] >>
 rpt strip_tac >>
-Cases_on `status` >> (
+Cases_on `status` >> Cases_on `scopes_stack` >> (
  fs [stmt_exec]
 ) >>
 Cases_on `is_v_bool e` >> (
@@ -536,7 +499,7 @@ Cases_on `is_v_bool e` >> (
   metis_tac [((valOf o find_clause_stmt_red) "stmt_cond3"), clause_name_def]
  ],
 
- Cases_on `e_exec ctx g_scope_list scopes_stack e` >> (
+ Cases_on `e_exec ctx g_scope_list (h::t) e` >> (
   fs []
  ) >>
  pairLib.PairCases_on `x` >>
@@ -552,11 +515,12 @@ stmt_exec_sound (stmt_block decl_list s)
 Proof
 fs [stmt_exec_sound] >>
 rpt strip_tac >>
-Cases_on `status` >> (
+Cases_on `status` >> Cases_on `scopes_stack` >> (
  fs [stmt_exec]
 ) >>
 rw [] >>
-metis_tac [((valOf o find_clause_stmt_red) "stmt_block_enter"), clause_name_def]
+irule ((valOf o find_clause_stmt_red) "stmt_block_enter") >>
+fs [clause_name_def]
 QED
 
 Theorem stmt_exec_sound_red:
@@ -568,11 +532,9 @@ rpt strip_tac >| [
  (* Empty statement *)
  fs [stmt_exec_sound] >>
  rpt strip_tac >>
- Cases_on `status` >> (
+ Cases_on `status` >> Cases_on `scopes_stack` >> (
   fs [stmt_exec]
- ) >>
- (* TODO: Block exit? *)
- cheat,
+ ),
 
  (* Extern *)
  fs [stmt_ext_exec_sound_red],
@@ -589,11 +551,10 @@ rpt strip_tac >| [
  (* Apply statement *)
  fs [stmt_app_exec_sound_red],
 
- (* Assign statement *)
- (* TODO *)
+ (* TODO: Assign statement *)
  fs [stmt_ass_exec_sound_red],
 
- (* Sequence of statements *)
+ (* TODO: Sequence of statements *)
  fs [stmt_seq_exec_sound_red],
 
  (* Conditional statement *)
